updates

generic/Zeta.Generic.Interleave.fst
@@ -1,12 +1,37 @@
 module Zeta.Generic.Interleave
 
+open FStar.Classical
+module SS = Zeta.SSeq
+
+#push-options "--fuel 0 --ifuel 1 --query_stats"
+
+let apply_per_thread_prefix (#vspec:_) (#n:_) (il: verifiable_log vspec n) (i:nat{i <= length il})
+  : Lemma (ensures (let ss = s_seq il in
+                    let il' = prefix il i in
+                    let ss' = s_seq il' in
+                    ss' `SS.sseq_all_prefix_of` ss))
+          [SMTPat (prefix il i)]
+  = per_thread_prefix il i
+
 let lemma_prefix_verifiable (#vspec:_) (n:_) (il:verifiable_log vspec n) (i:nat{i <= S.length il}):
-  Lemma (ensures (verifiable (I.prefix il i)))
-  = admit()
+  Lemma (ensures (verifiable (prefix il i)))
+  = let il' = prefix il i in
+    let gl' = s_seq il' in
+    let gl = s_seq il in
+    let aux (t:_)
+      : Lemma (ensures (T.verifiable (t, S.index gl' t)))
+      = let tl = G.index gl t in
+        let tl' = t,S.index gl' t in
+        eliminate
+        forall tid. (S.index gl' tid) `prefix_of` (S.index gl tid)
+        with t;
+        T.verifiable_implies_prefix_verifiable tl (T.length tl')
+    in
+    forall_intro aux
 
 let clock_prefix_prop (#vspec #n:_) (il: verifiable_log vspec n) (i: seq_index il) (j:nat{j <= length il /\ j > i})
   : Lemma (ensures (clock il i = clock (prefix il j) i))
-  = admit()
+  = ()
 
 //#push-options "--query_stats --debug Zeta.Generic.Interleave --debug_level SMTQuery"
 let lemma_cur_thread_state_extend (#vspec: verifier_spec) (#n:_)
@@ -14,9 +39,12 @@ let lemma_cur_thread_state_extend (#vspec: verifier_spec) (#n:_)
   : Lemma (ensures (let st_pre = cur_thread_state_pre il i in
                     let st_post = cur_thread_state_post il i in
                     st_post == V.verify_step (I.index il i) st_pre))
-  = admit()
+  = let il_post = prefix il (i+1) in
+    let il_pre = prefix il i in
 
+  admit()
 //#pop-options
+
 let lemma_non_cur_thread_state_extend (#vspec: verifier_spec) (#n:_) (tid: nat{tid < n})
   (il: verifiable_log vspec n) (i: seq_index il)
   : Lemma (requires (tid <> src il i))
@@ -80,82 +108,3 @@ let appfn_calls_snoc (#app #n:_) (il: verifiable_log app n {length il > 0})
                     | RunApp _ _ _ -> cr == SA.append1 cr' (to_app_fcr il i)
                     | _ -> cr == cr'))
   = admit()
-(*
-let idxfn_base #vspec #n #b (tfn: T.idxfn_t vspec b)
-  (il: verifiable_log vspec n) (i: seq_index il)
-  : b
-  = G.idxfn #vspec tfn (to_glog il) (i2s_map il i)
-
-val idxn_has_prefix_prop (#vspec:_) (#n:nat) (#b:_) (tfn: T.idxfn_t vspec b)
-  : Lemma (ensures (IF.prefix_property #(gen_seq vspec n) (idxfn_base #_ #n #_ tfn)))
-          [SMTPat (idxfn_base #_ #n #_ tfn)]
-
-let idxfn #b #vspec #n (tfn: T.idxfn_t vspec b)
-  : IF.idxfn_t (gen_seq vspec n) _
-  = idxfn_base tfn
-
-let idxfn_il_base #vspec #n (#b:eqtype) (tfn: T.idxfn_t vspec b)
-  (il: verifiable_log vspec n) (i: seq_index il)
-  : elem_src b n
-  = {e = idxfn tfn il i; s = src il i}
-
-let idxfn_il (#b:eqtype) #vspec #n (tfn: T.idxfn_t vspec b)
-  : IF.idxfn_t (gen_seq vspec n) _
-  = idxfn_il_base tfn
-
-(* this should be =() proof but does not work since some pattern matching does not kick-in *)
-val idxfn_prefix_property (#vspec:_) (#n:_) (#b:_) (tfn: T.idxfn_t vspec b)
-  (il: verifiable_log vspec n) (j:nat{j <= S.length il}) (i: nat{i < j})
-  : Lemma (ensures (idxfn tfn il i == idxfn tfn (prefix il j) i))
-          [SMTPat (idxfn tfn (prefix il j) i)]
-
-val idxfnil_prefix_property (#vspec:_) (#n:_) (#b:eqtype) (tfn: T.idxfn_t vspec b)
-  (il: verifiable_log vspec n) (j:nat{j <= S.length il}) (i: nat{i < j})
-  : Lemma (ensures (idxfn_il tfn il i == idxfn_il tfn (prefix il j) i))
-          [SMTPat (idxfn_il tfn (prefix il j) i)]
-
-let cond_idxfn_base #vspec #n #b #f (m: T.cond_idxfn_t b f)
-  (il: verifiable_log vspec n) (i: seq_index il{idxfn f il i})
-  = G.cond_idxfn m (to_glog il) (i2s_map il i)
-
-val cond_idxfn_has_prefix_prop (#vspec #n #b #f:_) (m: T.cond_idxfn_t b f)
-  : Lemma (ensures (IF.cond_prefix_property #(gen_seq vspec n) #_ #(idxfn f) (cond_idxfn_base m)))
-          [SMTPat (cond_idxfn_base #vspec #n #b #f m)]
-
-let cond_idxfn (#vspec #n #b #f:_) (m: T.cond_idxfn_t b f)
-  : IF.cond_idxfn_t b (idxfn f)
-  = cond_idxfn_base #vspec #n m
-
-let cond_idxfn_il_base #vspec #n (#b:eqtype) #f (m: T.cond_idxfn_t b f)
-  (il: verifiable_log vspec n) (i: seq_index il{idxfn f il i})
-  : elem_src b n
-  = {e = cond_idxfn m il i; s = src il i}
-
-let cond_idxfn_il #vspec #n (#b:eqtype) #f (m: T.cond_idxfn_t b f)
-  : IF.cond_idxfn_t (elem_src b n) (idxfn f)
-  = cond_idxfn_il_base #vspec #n #b #f m
-
-val lemma_cond_idxfn (#vspec #n:_) (#b: eqtype) (f:_) (m: T.cond_idxfn_t b f)
-  (il: verifiable_log vspec n)
-  : Lemma (ensures (let fm_il = to_fm (idxfn f) (cond_idxfn_il #vspec #n #_ #_ m) in
-                    let ilb = IF.filter_map fm_il il in
-                    let fm_s = to_fm (idxfn f) (cond_idxfn #vspec #n #_ #_ m) in
-                    let sb = IF.filter_map fm_s il in
-                    sb = i_seq ilb))
-
-val lemma_filter_map (#vspec #n:_) (#b:eqtype) (#f:_) (m: T.cond_idxfn_t b f)
-    (il: verifiable_log vspec n) (i: seq_index il)
-  : Lemma (ensures (let fmil = to_fm (idxfn f) (cond_idxfn_il #vspec #n #_ #_ m) in
-                    let ilb = IF.filter_map fmil il in
-                    let fm = to_fm f m in
-                    let ssb = SF.filter_map (G.gen_sseq vspec) fm (to_glog il) in
-                    ssb = s_seq ilb))
-
-val lemma_cond_idxfn_interleave (#vspec #n:_) (#b: eqtype) (#f:_) (m: T.cond_idxfn_t b f)
-  (il: verifiable_log vspec n)
-  : Lemma (ensures (let fm_s = to_fm (idxfn f) (cond_idxfn #vspec #n #_ #_ m) in
-                    let sb = IF.filter_map fm_s il in
-                    let fm = to_fm f m in
-                    let ssb = SF.filter_map (G.gen_sseq vspec) fm (to_glog il) in
-                    I.interleave #b sb ssb))
-*)
